Add more heap support, finish proof of list reverse example

coq/playground/himp/evaluator.v
@@ -5,122 +5,117 @@ Require Import ZArith.
 Require Import String.
 Require Import List.
 
-Fixpoint str_split k {V} m : option (V * Map string V) :=
+Set Implicit Arguments.
+
+Section MapSplit.
+  Variable K : Type.
+  Variable k_dec : forall (x y : K), {x=y}+{x<>y}.
+
+  Fixpoint map_split k {V} m : option (V * Map K V) :=
   match m with
     | mapEmpty => None
-    | (k' |-> v) => if string_dec k k' then Some (v, mapEmpty) else None
+    | (k' |-> v) => if k_dec k k' then Some (v, mapEmpty) else None
     | (l :* r) =>
-      match str_split k l with
+      match map_split k l with
         | Some (v, mapEmpty) => Some (v, r)
         | Some (v, l') => Some (v, l' :* r)
         | None =>
-          match str_split k r with
+          match map_split k r with
             | Some (v, r') => Some (v, l :* r')
             | None => None
           end
       end
   end.
+  Functional Scheme map_split_ind := Induction for map_split Sort Prop.
 
-Functional Scheme str_split_ind := Induction for str_split Sort Prop.
+  Lemma map_split_sound k {V} (m : Map K V) :
+    match map_split k m with
+      | Some (v, m') => m ~= k |-> v :* m'
+      | None => True
+    end.
+  Proof.
+  functional induction (map_split k m);auto;try equate_maps;
+  match goal with [H : map_split ?x ?m = _, IH : match map_split ?x ?m with None => _ | _ => _ end
+                   |- _] => rewrite H in IH; rewrite IH end;
+  equate_maps.
+  Qed.
 
-Lemma str_split_sound k {V} (m : Map string V) :
-  match str_split k m with
-    | Some (v, m') => m ~= k |-> v :* m'
-    | None => True
-  end.
-Proof.
-functional induction (str_split k m);auto;try equate_maps;
-match goal with [H : str_split ?x ?m = _, IH : match str_split ?x ?m with None => _ | _ => _ end
-              |- _] => rewrite H in IH; rewrite IH end;
-equate_maps.
-Qed.
+  Lemma map_split_sound' k {V} (v : V) m m' :
+    map_split k m = Some (v, m') -> m ~= k |-> v :* m'.
+  Proof.
+    pose proof (map_split_sound k m).
+    intro.
+    rewrite H0 in H.
+    assumption.
+  Qed.
 
-Lemma str_split_sound' k {V} (v : V) m m' :
-  str_split k m = Some (v, m') -> m ~= k |-> v :* m'.
-Proof.
-pose proof (str_split_sound k m).
-intro.
-rewrite H0 in H.
-assumption.
-Qed.
-
-Inductive HasKey {K V} (x : K) : Map K V -> Prop :=
+  Inductive HasKey (x : K) {V} : Map K V -> Prop :=
   | key_here : forall v, HasKey x (x |-> v)
   | key_left : forall env env', HasKey x env -> HasKey x (env :* env')
   | key_right : forall env env', HasKey x env' -> HasKey x (env :* env')
   .
 
-Lemma transport_has_key {K V} x (env env' : Map K V) :
-  env ~= env' -> (HasKey x env <-> HasKey x env').
-Proof.
-induction 1; split;intros;
-repeat match goal with [H : HasKey _ ?V |- _] => (is_var V;fail 1) || (inversion H; clear H; subst) end;
-repeat match goal with [H : _ <-> _ |- _] => destruct H end;
-eauto using key_left, key_right, key_here.
-Qed.
+  Lemma transport_has_key x {V} (env env' : Map K V) :
+    env ~= env' -> (HasKey x env <-> HasKey x env').
+  Proof.
+    induction 1; split;intros;
+    repeat match goal with [H : HasKey _ ?V |- _] => (is_var V;fail 1) || (inversion H; clear H; subst) end;
+    repeat match goal with [H : _ <-> _ |- _] => destruct H end;
+    eauto using key_left, key_right, key_here.
+  Qed.
 
-Definition has_key {K V} (x : K) (m : Map K V) :=
-  exists v env', m ~= x |-> v :* env'.
+  Definition has_key (x : K) {V} (m : Map K V) :=
+    exists v env', m ~= x |-> v :* env'.
 
-Lemma rep {K V} x (env : Map K V) :
-  has_key x env -> HasKey x env.
-Proof.
-destruct 1 as [v [env' H]].
-apply (transport_has_key x) in H.
-apply H.
-eauto using key_left, key_right, key_here.
-Qed.
+  Lemma rep x {V} (env : Map K V) :
+    has_key x env -> HasKey x env.
+  Proof.
+    destruct 1 as [v [env' H]].
+    apply (transport_has_key x) in H.
+    apply H.
+    eauto using key_left, key_right, key_here.
+  Qed.
 
-Lemma rep_inv {K V} x (env : Map K V) :
-  HasKey x env -> has_key x env.
-induction 1.
-eexists. eexists. symmetry. apply equivUnit.
-destruct IHHasKey as [v [env'' IH]].
-exists v. exists (env'' :* env').
-rewrite IH. equate_maps.
-destruct IHHasKey as [v [env'' IH]].
-exists v. exists (env :* env'').
-rewrite IH. equate_maps.
-Qed.
+  Lemma rep_inv x {V} (env : Map K V) :
+    HasKey x env -> has_key x env.
+    induction 1.
+    eexists. eexists. symmetry. apply equivUnit.
+    destruct IHHasKey as [v [env'' IH]].
+    exists v. exists (env'' :* env').
+    rewrite IH. equate_maps.
+    destruct IHHasKey as [v [env'' IH]].
+    exists v. exists (env :* env'').
+    rewrite IH. equate_maps.
+  Qed.
 
-Lemma lemm1 {K V} x :
-  @has_key K V x mapEmpty -> False.
-intros.
-apply rep in H.
-inversion H.
-Qed.
+  (* Without enforcing definedness there might be duplicate labels, but str_split finds some label *)
+  Lemma map_split_completeish : forall x {V} (env : Map K V),
+    has_key x env -> if map_split x env then True else False.
+  Proof.
+    induction env; intros; apply rep in H; inversion H; subst; simpl;
+    repeat match goal with
+        | [|- if if k_dec ?x ?y then _ else _ then _ else _] => destruct (k_dec x y);auto
+        | [|- if match map_split ?x ?env with  _ => _ end then _ else _] =>
+          destruct (map_split x env) as [[? []]|];auto using rep_inv
+    end.
+  Qed.
+End MapSplit.
 
-Lemma lemm2 {K V} x v x2 : @has_key K V x2 (x |-> v) -> x = x2.
-Proof.
-intros. apply rep in H.
-inversion H. auto.
-Qed.
-
-Lemma lemm3 {K V} x (env1 env2 : Map K V) :
-  has_key x (env1 :* env2) -> has_key x env1 \/ has_key x env2.
-Proof.
-intros.
-apply rep in H.
-inversion H; subst;
-auto using rep_inv.
-Qed.
-
-(* Without enforcing definedness there might be duplicate labels, but str_split finds some label *)
-Lemma str_split_completeish : forall x {V} (env : Map string V),
-  has_key x env -> if str_split x env then True else False.
-Proof.
-intros.
-induction env.
-
-apply lemm1 in H. auto.
-apply lemm2 in H. simpl. destruct (string_dec x k); auto.
-apply lemm3 in H. simpl.
-destruct (str_split x env1).
-destruct p; destruct m; trivial.
-destruct (str_split x env2).
-destruct p. trivial.
-intuition.
-Qed.
+Definition str_split := map_split string_dec.
+Definition str_split_sound k V (m : Map string V) :
+       match str_split k m with
+       | Some (v, m') => m ~= k |-> v :* m'
+       | None => True
+       end
+ := map_split_sound string_dec k m.
+Definition str_split_sound' : 
+ forall k V v (m m' : Map string V),
+       str_split k m = Some (v, m') -> m ~= k |-> v :* m'
+ := map_split_sound' string_dec.
+Definition str_split_completeish
+ : forall x V (env : Map string V),
+       has_key x env -> if str_split x env then True else False
+ := map_split_completeish string_dec.
 
 Definition eval cfg : option kcfg :=
   match cfg with
@@ -138,7 +133,6 @@ Definition eval cfg : option kcfg :=
         | BCon b =>
           match rest with
             | (KFreezeB f :: rest') => exp_step (f (BCon b) :: rest')
-            | (KFreezer (Fif s1 s2) :: rest') => exp_step (kra (SIf (BCon b) s1 s2) rest')
             | _ => None
           end
         | EVar x => 
@@ -146,12 +140,25 @@ Definition eval cfg : option kcfg :=
             | None => None
             | Some (v,env') => Some (KCfg (kra (ECon v) rest) (x |-> v :* env') heap lenv)
           end
+        | ELoad (ECon i) =>
+          match map_split Z.eq_dec i heap with
+            | None => None
+            | Some (j, _) => Some (KCfg (kra (ECon j) rest) env heap lenv)
+          end
+        | ELoad e => heat_step e (KFreezeE ELoad)
         | SAssign x (ECon i) =>
           match str_split x env with
             | None => None
-            | Some (_, env') => Some (KCfg (kra Skip rest) (x |-> i :* env') heap lenv)
+            | Some (_, env') => Some (KCfg rest (x |-> i :* env') heap lenv)
           end
         | SAssign x e => heat_step e (x :=□)
+        | HAssign (ECon i) (ECon j) =>
+          match map_split Z.eq_dec i heap with
+            | None => None
+            | Some (_, heap') => Some (KCfg rest env (i |-> j :* heap') lenv)
+          end
+        | HAssign (ECon i) e => heat_step e (FreezeR HAssign (ECon i))
+        | HAssign e e2 => heat_step e (FreezeL HAssign e2)
         | Jump l =>
           match str_split l lenv with
             | None => None
@@ -167,23 +174,24 @@ Definition eval cfg : option kcfg :=
           if Zneq_bool 0%Z j then exp1_step (ECon (Zdiv i j)) else None
         | EDiv (ECon i) e2       => heat_step e2 (ECon i /□)
         | EDiv e1 e2             => heat_step e1 (□/ e2)
+        | BNot (BCon b)          => exp1_step (BCon (negb b))
+        | BNot b                => heat_step b (KFreezeB BNot)
         | BLe (ECon i) (ECon j) => exp1_step (BCon (Zle_bool i j))
-        | BLe (ECon i) e2       => heat_step e2 (i <= □)
-        | BLe e1 e2             => heat_step e1 (□ <= e2)
+        | BLe (ECon i) e2       => heat_step e2 (i <=□)
+        | BLe e1 e2             => heat_step e1 (□<= e2)
+        | BEq (ECon i) (ECon j) => exp1_step (BCon (i =? j)%Z)
+        | BEq (ECon i) e2       => heat_step e2 (i ==□)
+        | BEq e1 e2             => heat_step e1 (□== e2)
         | BAnd (BCon b) be2 => if b then exp1_step be2 else exp1_step (BCon false)
-        | BAnd be1 be2 => heat_step be1 (□ && be2)
+        | BAnd be1 be2 => heat_step be1 (□&& be2)
         | Skip => exp_step rest
         | SIf (BCon b) s1 s2 => if b then exp1_step s1 else exp1_step s2
         | SIf be s1 s2 => heat_step be (if□then s1 else s2)
         | SWhile b s => exp1_step (SIf b (Seq s (SWhile b s)) Skip)
         | Seq s1 s2 => heat_step s1 s2
 
-        | KFreezer _ => None
         | KFreezeE _ => None
         | KFreezeB _ => None
-         (* unimplemented *)
-        | BNot _ => None
-        | HAssign _ _ => None
       end
 end.
 
@@ -191,9 +199,10 @@ Functional Scheme eval_ind := Induction for eval Sort Prop.
 
 Lemma eval_sound : forall cfg, match eval cfg with Some cfg' => kstep cfg cfg' | None => True end.
 Proof.
-intros.
-functional induction (eval cfg);try econstructor(reflexivity || assumption ||
-match goal with [H : str_split _ _ = _ |- _] => apply str_split_sound' in H;eassumption end).
+intros;functional induction (eval cfg);unfold str_split in * |-;
+repeat match goal with
+  [H : map_split _ _ _ = _ |- _] => apply map_split_sound' in H end;
+econstructor(reflexivity || eassumption).
 Qed.
 
 Lemma eval_completeish : forall cfg cfg', kstep cfg cfg' ->
@@ -201,19 +210,19 @@ Lemma eval_completeish : forall cfg cfg', kstep cfg cfg' ->
                                                          Some cfg'' => kstep cfg cfg''
                                                        | None => False end.
 Proof.
-Ltac good_split x env :=
+Ltac good_split H dec x env :=
   let H0 := fresh in
-  assert (has_key x env) as H0 by firstorder;
-  apply str_split_completeish in H0;
-  pose proof (str_split_sound x env);
-  destruct (str_split x env) as [[]|];[clear H0|solve[destruct H0]].
+  assert (has_key x env) as H0 by (clear -H;firstorder);
+  apply (map_split_completeish dec) in H0;
+  pose proof (map_split_sound dec x env);
+  destruct (map_split dec x env) as [[]|];[clear H0|solve[destruct H0]].
 
-intros;destruct H;simpl;repeat match goal with
-  | [H : ?env ~= ?x |-> _ :* _ |- context [match str_split ?x ?env with None => _ | _ => _ end]] =>
-    good_split x env
+intros;destruct H eqn:?;simpl;unfold str_split in *|-*;try solve[repeat match goal with
+  | [H : ?env ~= ?x |-> _ :* _ |- context [match map_split ?dec ?x ?env with None => _ | _ => _ end]] =>
+    good_split H dec x env
   | [|- kstep _ _] => econstructor (eassumption || reflexivity)
   | [H : Zneq_bool ?x ?y = _ |- context [if Zneq_bool ?x ?y then _ else _]] => rewrite H
   | [|- context [match ?e with EVar _ => _ | _ => _ end]] => destruct e; try discriminate
   | [|- context [match ?b with BCon _ => _ | _ => _ end]] => destruct b; try discriminate
-end.
+end].
 Qed.
