coq/playground/himp/simple_proofs.v
@@ -5,36 +5,135 @@ Require Import String.
 Open Scope string_scope.
 
 Require Import domains.
+Require Import kstyle.
+Require Import evaluator.
 
-Lemma eval_happy : forall env,
-  steps (KCfg (kra (SAssign "x" (EPlus (EVar "x") (EVar "y"))) nil)
-            (env :* "x" |-> 12%Z :* "y" |-> 13%Z) mapEmpty mapEmpty)
-        (KCfg nil (env :* "x" |-> 25%Z :* "y" |-> 13%Z) mapEmpty mapEmpty).
-intros.
-repeat (refine (more _ (@kequiv_refl _) _ _);[econstructor (reflexivity || find_map_entry)|]);
-simpl Zplus; finish.
-Qed.
+Coercion EVar : string >-> Exp.
+Coercion ECon : Z >-> Exp.
 
-(* Try "quote" on the env *)
-(* Use a mixed coinductive sequencing to use loop invariants? *)
-
-Lemma eval_happy' : forall env,
-  steps (KCfg (kra (SAssign "x" (EPlus (EVar "x") (EVar "y"))) nil)
-            ("x" |-> 12%Z :* "y" |-> 13%Z :* env) mapEmpty mapEmpty)
-        (KCfg nil ("x" |-> 25%Z :* "y" |-> 13%Z :* env) mapEmpty mapEmpty).
-intros;
-repeat (refine (more _ (@kequiv_refl _) _ _);[match goal with [|- kstep ?l _] => eapply (eval_sound l) end|]);
-simpl Zplus; finish.
-Qed.
-
-Lemma loop_test':
-  steps (KCfg (kra (SWhile (BLe (ECon 0) (EVar "x"))
-    (SAssign "x" (EPlus (EVar "x") (ECon (-1)%Z))))
-  nil) ("x" |-> 25%Z) mapEmpty mapEmpty)
-  (KCfg nil ("x" |-> (-1)%Z) mapEmpty mapEmpty).
+Lemma heap_test : forall p env,
+  steps (KCfg (kra (HAssign "x" (EPlus (ELoad "x") 1%Z)) nil)
+              (env :* "x" |-> p) (p |-> 12%Z) mapEmpty)
+        (KCfg nil (env :* "x" |-> p) (p |-> 13%Z) mapEmpty).
 Proof.
-Ltac step_eval :=refine (more _ (@kequiv_refl _) _ _);[match goal with [|- kstep ?l _] => eapply (eval_sound l) end|].
-intros;repeat step_eval;simpl;finish.
+intros.
+repeat (refine (more _ (@kequiv_refl _) _ _);[econstructor(reflexivity||find_map_entry)|]).
+finish.
+Qed.
+
+Definition listrev :=
+  (SWhile (BNot (BEq 0%Z "p"))
+     (Seq (SAssign "next" (ELoad (EPlus "p" 1%Z)))
+     (Seq (HAssign (EPlus "p" 1%Z) "q")
+     (Seq (SAssign "q" "p")
+          (SAssign "p" "next"))))).
+
+Fixpoint listrep (l : list Z) (p : Z) (m : Map Z Z) : Prop :=
+  match l with
+    | nil => p = 0%Z /\ m ~= mapEmpty
+    | (v :: l') =>
+       p <> 0%Z /\
+       exists next m',
+         m ~= p |-> v :* (p + 1)%Z |-> next :* m'
+         /\ listrep l' next m'
+  end.
+
+Ltac same_eprefix H :=
+  match goal with
+      [ H : exists _ : ?A , _ |- exists _ : ?A , _ ] =>
+      let x := fresh "x" in destruct H as [x H]; exists x
+  end.
+  
+Lemma listrep_equiv : forall l p m m', m ~= m' -> listrep l p m -> listrep l p m'.
+destruct l;simpl; intuition.
+rewrite <- H; assumption.
+repeat same_eprefix H2.
+intuition.
+rewrite <- H; assumption.
+Qed.
+
+Lemma rev_test : forall lenv,
+  steps (KCfg (kra listrev nil)
+              ("p" |-> 1 :* "q" |-> 0 :* "next" |-> 1)%Z
+              (1 |-> 12 :* 2 |-> 3 :*
+               3 |-> 13 :* 4 |-> 5 :*
+               5 |-> 14 :* 6 |-> 0)%Z
+              lenv)
+        (KCfg nil
+              ("p" |-> 0 :* "q" |-> 5 :* "next" |-> 0)%Z
+              (1 |-> 12 :* 2 |-> 0 :*
+               3 |-> 13 :* 4 |-> 1 :*
+               5 |-> 14 :* 6 |-> 3)%Z
+              lenv).
+Proof.
+intros;repeat step_rule;finish.
+Qed.
+
+(* For a generic statement about reverse, we would like
+   to have an existential about the address the reversed
+   list starts at, need a different sort of reaching
+   to let us put the existential where we like. *)
+
+CoInductive reaches (s : kcfg) (phi : kcfg -> Prop) : Prop :=
+ | r_done : phi s -> reaches s phi
+ | r_more : forall s', kstep s s' -> reaches s' phi -> reaches s phi.
+
+Lemma rev_pf : forall p l q l' heap0 heap_l heap_l' lenv,
+  listrep l p heap_l ->
+  listrep l' q heap_l' ->
+  heap0 ~= heap_l :* heap_l' ->
+  reaches (KCfg (kra listrev nil)
+                ("p" |-> p :* "next" |-> p :* "q" |-> q)
+                heap0
+                lenv)
+          (fun cfg' =>
+             exists q' heap',
+               listrep (rev_append l l') q' heap' /\
+               kequiv cfg'
+                      (KCfg nil
+                            ("p" |-> 0 :* "next" |-> 0 :* "q" |-> q')%Z
+                            heap'
+                            lenv)).
+Proof.
+cofix.
+intros.
+Ltac r_step := (eapply r_more;[solve[econstructor(reflexivity||find_map_entry)]|]).
+r_step.
+Ltac rsplit_if :=
+  cbv beta; match goal with
+      | [|- reaches (KCfg (kra (KStmt (SIf (BCon ?test) _ _)) _) _ _ _) _] => split_bool test
+  end.
+repeat ((eapply rev_pf;fail 1) || (r_step || rsplit_if)).
+(* zero case *)
+clear rev_pf.
+apply r_done.
+exists q. exists heap0.
+split;[|subst;reflexivity].
+(* show l is nil *)
+destruct l;destruct H;[|solve[exfalso;auto]].
+simpl.
+revert H0.
+apply listrep_equiv.
+rewrite H1, H2. equate_maps.
+
+(* Nonzero case *)
+(* Stuck on a lookup that needs domain reasoning to go through *)
+(* exclude nil l*)
+destruct l. (* nil *) contradict n. clear -H. destruct H. auto.
+destruct H as [_ [next [m' [pequiv p_rel_l]]]].
+rewrite pequiv in H1; clear pequiv.
+
+repeat ((eapply rev_pf;fail 1) || (r_step || rsplit_if)).
+simpl; eapply rev_pf.
+
+eassumption.
+split. congruence.
+eexists; eexists.
+split;[reflexivity|eassumption].
+equate_maps.
+apply equivJoin.
+reflexivity.
+apply equivComAssoc.
 Qed.
 
 Function evals n kcfg :=
@@ -46,6 +145,7 @@ Function evals n kcfg :=
       | None => kcfg
      end
   end.
+
 Lemma evals_sound :
   forall n c1 c2,
     kequiv (evals n c1) c2 -> steps c1 c2.
@@ -60,25 +160,17 @@ assumption. apply IHn. assumption.
 apply done.
 Qed.
 
-Lemma loop_test'':
-  steps (KCfg (kra (SWhile (BLe (ECon 0) (EVar "x"))
-    (SAssign "x" (EPlus (EVar "x") (ECon (-1)%Z))))
-  nil) ("x" |-> 25%Z) mapEmpty mapEmpty)
-  (KCfg nil ("x" |-> (-1)%Z) mapEmpty mapEmpty).
-Proof.
-intros;apply (evals_sound 1000);lazy;repeat (apply conj);[reflexivity|simpl;equate_maps ..].
+Lemma eval_happy : forall env,
+  steps (KCfg (kra (SAssign "x" (EPlus "x" "y")) nil)
+            (env :* "x" |-> 12%Z :* "y" |-> 13%Z) mapEmpty mapEmpty)
+        (KCfg nil (env :* "x" |-> 25%Z :* "y" |-> 13%Z) mapEmpty mapEmpty).
+intros.
+repeat (refine (more _ (@kequiv_refl _) _ _);[econstructor (reflexivity || find_map_entry)|]);
+simpl Zplus; finish.
 Qed.
 
-Lemma loop_test:
-  steps (KCfg (kra (SWhile (BLe (ECon 0) (EVar "x"))
-    (SAssign "x" (EPlus (EVar "x") (ECon (-1)%Z))))
-  nil) ("x" |-> 25%Z) mapEmpty mapEmpty)
-  (KCfg nil ("x" |-> (-1)%Z) mapEmpty mapEmpty).
-Proof.
-intros;
-repeat (refine (more _ (@kequiv_refl _) _ _);[econstructor (reflexivity || find_map_entry)|];instantiate;simpl Zplus);
-finish.
-Qed.
+(* Try "quote" on the env *)
+(* Use a mixed coinductive sequencing to use loop invariants? *)
 
 CoFixpoint sum :
   forall (x y z : Z) erest env heap labels,
@@ -86,18 +178,25 @@ CoFixpoint sum :
     z = (x + y)%Z ->
     env ~= ("i" |-> x :* "j" |-> y :* erest) ->
   steps
-    (KCfg (kra (SWhile (BLe (ECon 1%Z) (EVar "i"))
+    (KCfg (kra (SWhile (BLe 1%Z "i")
                        (Seq
-                          (SAssign "i" (EPlus (EVar "i") (ECon (-1)%Z)))
-                          (SAssign "j" (EPlus (EVar "j") (ECon 1%Z)))))
+                          (SAssign "i" (EPlus "i" (-1)%Z))
+                          (SAssign "j" (EPlus "j" 1%Z))))
                kdot)
                 env heap labels)
     (KCfg kdot
           ("i" |-> 0%Z :* "j" |-> z%Z :* erest) heap labels).
-intros;step_rule;run_circ sum.
+intros; step_rule;run_circ sum.
 Qed.
 
-Coercion EVar : string >-> Exp.
+Lemma eval_happy' : forall env,
+  steps (KCfg (kra (SAssign "x" (EPlus "x" "y")) nil)
+            ("x" |-> 12%Z :* "y" |-> 13%Z :* env) mapEmpty mapEmpty)
+        (KCfg nil ("x" |-> 25%Z :* "y" |-> 13%Z :* env) mapEmpty mapEmpty).
+intros;
+repeat (refine (more _ (@kequiv_refl _) _ _);[match goal with [|- kstep ?l _] => eapply (eval_sound l) end|]);
+simpl Zplus; finish.
+Qed.
 
 Definition gcdProg : Map string Stmt :=
   "gcd" |->
@@ -114,4 +213,35 @@ Lemma label_eval : forall env,
         (KCfg (kra (Jump "done") kdot)
              ("a" |-> 1%Z :* "b" |-> 1%Z :* env) mapEmpty gcdProg).
 intros. apply evals_sound with 307; simpl; repeat split; reflexivity.
+Qed.
+
+(* Some performance tests *)
+Lemma loop_test:
+  steps (KCfg (kra (SWhile (BLe 0%Z "x")
+    (SAssign "x" (EPlus "x" (-1)%Z)))
+  nil) ("x" |-> 25%Z) mapEmpty mapEmpty)
+  (KCfg nil ("x" |-> (-1)%Z) mapEmpty mapEmpty).
+Proof.
+intros;
+repeat (refine (more _ (@kequiv_refl _) _ _);[econstructor (reflexivity || find_map_entry)|];instantiate;simpl Zplus);
+finish.
+Qed.
+
+Lemma loop_test':
+  steps (KCfg (kra (SWhile (BLe 0%Z "x")
+    (SAssign "x" (EPlus "x" (-1)%Z)))
+  nil) ("x" |-> 25%Z) mapEmpty mapEmpty)
+  (KCfg nil ("x" |-> (-1)%Z) mapEmpty mapEmpty).
+Proof.
+Ltac step_eval :=refine (more _ (@kequiv_refl _) _ _);[match goal with [|- kstep ?l _] => eapply (eval_sound l) end|].
+intros;repeat step_eval;simpl;finish.
+Qed.
+
+Lemma loop_test'':
+  steps (KCfg (kra (SWhile (BLe (ECon 0) (EVar "x"))
+    (SAssign "x" (EPlus (EVar "x") (ECon (-1)%Z))))
+  nil) ("x" |-> 25%Z) mapEmpty mapEmpty)
+  (KCfg nil ("x" |-> (-1)%Z) mapEmpty mapEmpty).
+Proof.
+intros;apply (evals_sound 1000);lazy;repeat (apply conj);[reflexivity|simpl;equate_maps ..].
 Qed.
